verify that parseSector returns a valid pivot node

disk-betree/ByteBetree.dfy
@@ -10,11 +10,14 @@ module Marshalling {
   import opened NativeTypes
   import opened Sequences
   import BC = BetreeGraphBlockCache
-  import BT = PivotBetreeSpec
+  import BT = PivotBetreeSpec`Internal
   import M = ValueMessage
   import ReferenceType`Internal
   import LBAType`Internal
   import ValueWithDefault`Internal
+  import Pivots = PivotsLib
+  import MS = MapSpec
+  import Keyspace = MS.Keyspace
 
   type Reference = BC.Reference
   type LBA = BC.LBA
@@ -62,6 +65,8 @@ module Marshalling {
     GTaggedUnion([SuperblockGrammar(), PivotNodeGrammar()])    
   }
 
+  /////// Conversion to PivotNode
+
   function method valToReference(v: V) : Reference
   requires ValInGrammar(v, GUint64)
   {
@@ -82,6 +87,8 @@ module Marshalling {
 
   function method valToLBAsAndRefcounts(a: seq<V>) : Option<(map<Reference, LBA>, map<Reference, int>)>
   requires forall i | 0 <= i < |a| :: ValInGrammar(a[i], GTuple([GUint64, GUint64, GUint64]))
+  ensures var s := valToLBAsAndRefcounts(a) ; s.Some? ==> 0 !in s.value.0.Values
+  ensures var s := valToLBAsAndRefcounts(a) ; s.Some? ==> s.value.0.Keys == s.value.1.Keys
   {
     if |a| == 0 then
       Some((map[], map[]))
@@ -93,7 +100,7 @@ module Marshalling {
           var ref := valToReference(tuple.t[0]);
           var lba := valToLBA(tuple.t[1]);
           var refcount := valToInt(tuple.t[2]);
-          if ref in refcounts then (
+          if ref in refcounts || lba == 0 then (
             None
           ) else (
             Some((lbas[ref := lba], refcounts[ref := refcount]))
@@ -106,6 +113,7 @@ module Marshalling {
 
   function method valToSuperblock(v: V) : Option<BC.Superblock>
   requires ValInGrammar(v, SuperblockGrammar())
+  ensures var s := valToSuperblock(v) ; s.Some? ==> BC.WFSuperblock(BC.Constants(), s.value)
   {
     var res := valToLBAsAndRefcounts(v.a);
     match res {
@@ -120,20 +128,22 @@ module Marshalling {
     Some(M.Define(v.b))
   }
 
-  function method valToKeyMessageMap(a: seq<V>) : Option<Bucket>
+  function method valToKeyMessageMap(a: seq<V>, pivotTable: seq<Key>, i: int) : Option<Bucket>
   requires forall i | 0 <= i < |a| :: ValInGrammar(a[i], GTuple([GByteArray, MessageGrammar()]))
+  requires Pivots.WFPivots(pivotTable)
+  ensures var s := valToKeyMessageMap(a, pivotTable, i) ; s.Some? ==> forall key | key in s.value :: Pivots.Route(pivotTable, key) == i
   {
     if |a| == 0 then
       Some(map[])
     else (
-      var res := valToKeyMessageMap(DropLast(a));
+      var res := valToKeyMessageMap(DropLast(a), pivotTable, i);
       match res {
         case Some(m) => (
           var tuple := Last(a);
           assert ValInGrammar(tuple, GTuple([GByteArray, MessageGrammar()]));
           var key := tuple.t[0].b;
           var msg := valToMessage(tuple.t[1]);
-          if key in m then (
+          if key in m || Pivots.Route(pivotTable, key) != i then (
             None
           ) else (
             Some(m[key := msg.value])
@@ -144,10 +154,11 @@ module Marshalling {
     )
   }
 
-  function method valToBucket(v: V) : Option<Bucket>
+  function method valToBucket(v: V, pivotTable: seq<Key>, i: int) : Option<Bucket>
   requires ValInGrammar(v, BucketGrammar())
+  requires Pivots.WFPivots(pivotTable)
   {
-    valToKeyMessageMap(v.a)
+    valToKeyMessageMap(v.a, pivotTable, i)
   }
 
   function method valToKey(v: V) : Key
@@ -158,13 +169,26 @@ module Marshalling {
 
   function method valToPivots(a: seq<V>) : Option<seq<Key>>
   requires forall i | 0 <= i < |a| :: ValInGrammar(a[i], GByteArray)
+  ensures var s := valToPivots(a) ; s.Some? ==> Pivots.WFPivots(s.value)
   {
     if |a| == 0 then
       Some([])
     else
       match valToPivots(DropLast(a)) {
         case None => None
-        case Some(pref) => Some(pref + [valToKey(Last(a))])
+        case Some(pref) => (
+          var key := valToKey(Last(a));
+
+          if (|key| != 0 && (|pref| > 0 ==> Keyspace.lt(Last(pref), key))) then (
+            Keyspace.reveal_seq_lte();
+            Keyspace.IsNotMinimum([], key);
+            Keyspace.StrictlySortedAugment(pref, key);
+
+            Some(pref + [key])
+          ) else (
+            None
+          )
+        )
       }
   }
 
@@ -180,16 +204,19 @@ module Marshalling {
       }
   }
 
-  function method valToBuckets(a: seq<V>) : Option<seq<Bucket>>
+  function method valToBuckets(a: seq<V>, pivotTable: seq<Key>) : Option<seq<Bucket>>
+  requires Pivots.WFPivots(pivotTable)
   requires forall i | 0 <= i < |a| :: ValInGrammar(a[i], BucketGrammar())
+  ensures var s := valToBuckets(a, pivotTable) ; s.Some? ==> |s.value| == |a|
+  ensures var s := valToBuckets(a, pivotTable) ; s.Some? ==> forall i | 0 <= i < |s.value| :: forall key | key in s.value[i] :: Pivots.Route(pivotTable, key) == i
   {
     if |a| == 0 then
       Some([])
     else (
-      match valToBuckets(DropLast(a)) {
+      match valToBuckets(DropLast(a), pivotTable) {
         case None => None
         case Some(pref) => (
-          match valToBucket(Last(a)) {
+          match valToBucket(Last(a), pivotTable, |pref|) {
             case Some(bucket) => Some(pref + [bucket])
             case None => None
           }
@@ -200,6 +227,7 @@ module Marshalling {
 
   function method {:fuel ValInGrammar,2} valToPivotNode(v: V) : Option<Node>
   requires ValInGrammar(v, PivotNodeGrammar())
+  ensures var s := valToPivotNode(v); s.Some? ==> BT.WFNode(s.value)
   {
     match valToPivots(v.t[0].a) {
       case None => None
@@ -207,8 +235,8 @@ module Marshalling {
         match valToChildren(v.t[1].a) {
           case None => None
           case Some(children) => (
-            if (|children| == 0 || |children| == |pivots| + 1) then (
-              match valToBuckets(v.t[2].a) {
+            if ((|children| == 0 || |children| == |pivots| + 1) && |v.t[2].a| == |pivots| + 1) then (
+              match valToBuckets(v.t[2].a, pivots) {
                 case None => None
                 case Some(buckets) => (
                   Some(BT.G.Node(pivots, if |children| == 0 then None else Some(children), buckets))
@@ -225,6 +253,10 @@ module Marshalling {
 
   function method valToSector(v: V) : Option<Sector>
   requires ValInGrammar(v, SectorGrammar())
+  ensures var s := valToSector(v);
+      s.Some? && s.value.SectorSuperblock? ==> BC.WFSuperblock(BC.Constants(), s.value.superblock)
+  ensures var s := valToSector(v);
+      s.Some? && s.value.SectorBlock? ==> BT.WFNode(s.value.block)
   {
     if v.c == 0 then (
       match valToSuperblock(v.val) {
@@ -241,6 +273,11 @@ module Marshalling {
 
   function method {:opaque} parseSector(data: seq<byte>) : Option<Sector>
   requires |data| < 0x1_0000_0000_0000_0000;
+  ensures var s := parseSector(data);
+      s.Some? && s.value.SectorSuperblock? ==> BC.WFSuperblock(BC.Constants(), s.value.superblock)
+  ensures var s := parseSector(data);
+      s.Some? && s.value.SectorBlock? ==> BT.WFNode(s.value.block)
+
   {
     match parse_Val(data, SectorGrammar()).0 {
       case Some(v) => valToSector(v)
